refactor() move solutions to 'davi' folder to avoid conflicts

davi_solutions/Ex4.dfy
@@ -10,46 +10,49 @@ module Ex4 {
     ghost var content : set<nat>
 
     ghost function Valid() : bool 
-      reads this, footprint, this.list
+      reads this, this.footprint, this.list
     {
       if (this.list == null)
         then 
-          footprint == {}
+          this.footprint == {}
           &&
-          content == {}
+          this.content == {}
         else 
-          footprint == list.footprint
+          this.footprint == list.footprint
           &&
-          content == list.content
+          this.content == list.content
           &&
           list.Valid()
     }
 
-    constructor () 
-      ensures Valid() && this.content == {} && this.footprint == {}
+    constructor() 
+      ensures Valid() 
+        && this.content == {} 
+        && this.footprint == {} 
+        && this.list == null
     {
       list := null; 
       footprint := {}; 
       content := {};      
     }
 
-
-    method mem (v : nat) returns (b : bool)
+    method mem(v : nat) returns (b : bool)
       requires this.Valid()
       ensures b == (v in this.content)
     {
       b := false;
-      if list != null{      
+      if (list != null) {
         b := this.list.mem(v);
       }
     }
 
-    method add (v : nat) 
+    method add(v : nat) 
       requires this.Valid()
-      ensures this.content == { v } + old(this.content)
-      ensures this.footprint == { this.list } + old(this.footprint) 
-      modifies this
       ensures this.Valid()
+      ensures this.content == { v } + old(this.content)
+      ensures this.footprint == { this.list } + old(this.footprint)
+      ensures fresh(this.footprint - old(this.footprint))
+      modifies this
     {
       var value_exists := this.mem(v);
       if (this.list == null) {
@@ -58,105 +61,93 @@ module Ex4 {
         this.footprint := { aux };
         this.content := { v };
       } else if (!value_exists) {
-        var added_node := this.list.add(v);
-        this.list := added_node;
-        this.content := added_node.content;
-        this.footprint := added_node.footprint;
+        var aux := this.list.add(v);
+        this.list := aux;
+        this.content := aux.content;
+        this.footprint := aux.footprint;
       }
     }
-  
-method union(s: Set) returns (r: Set)
-  requires this.Valid()
-  requires s.Valid()
 
-  ensures r.Valid()
-  ensures r.content == this.content + s.content
-  ensures fresh(r)
-{
-  r := new Set();
+    method union(s : Set) returns (r : Set)
+      requires this.Valid()
+      requires s.Valid()
 
-  var curr := this.list;
-  ghost var seen_elements := {};
-
-  while (curr != null)
-    invariant r.Valid()
-    invariant curr != null ==> curr.Valid()
-    invariant curr != null && curr.next != null ==> curr.next.Valid()
-    invariant r.content == seen_elements
-    invariant curr != null ==> this.content == curr.content + seen_elements
-    invariant curr == null ==> this.content == seen_elements
-
-    decreases if curr != null then curr.footprint else {}
-  {
-    r.add(curr.val);
-    seen_elements := seen_elements + {curr.val};
-    curr := curr.next;
-  } 
-  assert seen_elements == this.content;
-
-  var curr_s := s.list;
-
-  ghost var seen_elements_s := {};
-
-  while (curr_s != null)
-      invariant r.Valid()
-      invariant curr_s != null ==> curr_s.Valid()
-      invariant curr_s != null && curr_s.next != null ==> curr_s.next.Valid()
-      invariant r.content == seen_elements_s + seen_elements
-      invariant curr_s != null ==> s.content == curr_s.content + seen_elements_s
-      invariant curr_s == null ==>  s.content == seen_elements_s 
-      
-      decreases if curr_s != null then curr_s.footprint else {}
-    {
-      r.add(curr_s.val);
-      seen_elements_s := seen_elements_s + {curr_s.val};
-      curr_s := curr_s.next;
-    }
-
-  assert seen_elements + seen_elements_s == this.content + s.content;
-}
-
-  method inter(s : Set) returns (r : Set)
-      requires this.Valid() 
-            && s.Valid()
       ensures r.Valid()
-      ensures r.content == this.content * s.content
+      ensures r.content == this.content + s.content
+      ensures |r.content| <= |this.content| + |s.content|
+      // ensures |r.footprint| >= |this.footprint| + |s.footprint| // to be proved
       ensures fresh(r)
     {
       r := new Set();
 
       var curr := this.list;
+      ghost var seen_elements := {};
+
+      while (curr != null) 
+        decreases if curr != null then curr.footprint else {}
+        invariant r.Valid()
+        invariant curr != null ==> curr.Valid()
+        invariant r.content == seen_elements
+        invariant curr != null ==> this.content == curr.content + seen_elements
+        invariant curr == null ==> this.content == seen_elements
+      {
+        r.add(curr.val);
+        seen_elements := seen_elements + { curr.val };
+        curr := curr.next;
+      }
+
+      var curr_s := s.list;
+      ghost var seen_elements_s := {};
+
+      while (curr_s != null) 
+        decreases if curr_s != null then curr_s.footprint else {}
+        invariant r.Valid()
+        invariant curr_s != null ==> curr_s.Valid()
+        invariant r.content == seen_elements_s + seen_elements
+        invariant curr_s != null ==> s.content == curr_s.content + seen_elements_s
+        invariant curr_s == null ==> s.content == seen_elements_s
+      {
+        r.add(curr_s.val);
+        seen_elements_s := seen_elements_s + { curr_s.val };
+        curr_s := curr_s.next;
+      }
+    }
+
+    method inter(s : Set) returns (r : Set)
+      requires this.Valid()
+      requires s.Valid()
+
+      ensures r.Valid()
+      ensures r.content == this.content * s.content
+      ensures fresh(r)
+    {
+      r := new Set();
+      var curr := this.list;
       ghost var added_elements := {};
       ghost var seen_elements := {};
 
-      while (curr != null)
+      while (curr != null) 
+        decreases if curr != null then curr.footprint else {}
         invariant r.Valid()
         invariant curr != null ==> curr.Valid()
-        invariant curr != null && curr.next != null ==> curr.next.Valid()
         invariant r.content == added_elements
         invariant curr != null ==> this.content == curr.content + seen_elements
         invariant curr == null ==> this.content == seen_elements
 
         invariant seen_elements * s.content == added_elements
-        
+
         invariant forall x :: x in added_elements ==> x in this.content
         invariant forall x :: x in added_elements ==> x in s.content
-
-        
-        decreases if curr != null then curr.footprint else {}
       {
         var also_in_s := s.mem(curr.val);
-        if (also_in_s == true){
+        if (also_in_s) {
           r.add(curr.val);
-          added_elements := added_elements + {curr.val};
+          added_elements := added_elements + { curr.val };
         }
-          seen_elements := seen_elements + {curr.val};
-          curr := curr.next;
-
-        
-      } 
+        seen_elements := seen_elements + { curr.val };
+        curr := curr.next;
+      }
     }
-
   }
-
 }
+
