davi_solutions/Ex5.dfy
@@ -4,11 +4,6 @@ module Ex5 {
   
   import Ex3=Ex3
 
-  function max(p1: nat, p2: nat): nat{
-      if p1>=p2 then p1
-      else p2
-  }
-
   class Set {
     var tbl : array<bool>  
     var list : Ex3.Node?
@@ -21,43 +16,36 @@ module Ex5 {
     ghost function Valid() : bool 
       reads this, this.footprint, this.list, this.tbl
     {
+      this.tbl.Length == |this.tblSeq|
+      &&
       if (this.list == null)
         then
-          |this.tblSeq| == this.tbl.Length
-          && 
           this.footprint == {}
           &&
           this.content == {}
           &&
-          (forall k :: 0 <= k < |this.tblSeq| ==> this.tblSeq[k] == false)
-          &&
-          forall k :: 0 <= k < |this.tblSeq| ==> this.tblSeq[k] == this.tbl[k]
+          forall k :: 0 <= k < |this.tblSeq| == this.tbl.Length ==> this.tblSeq[k] == this.tbl[k] == false
         else 
-          |this.tblSeq| == this.tbl.Length
-          && 
           this.footprint == this.list.footprint
-          && 
+          &&
           this.content == this.list.content
-          && 
+          &&
           this.list.Valid()
-          && 
-          (forall k :: 0 <= k < |this.tblSeq| ==> this.tblSeq[k] == this.tbl[k] == (k in this.content))
+          &&
+          (forall n :: n in this.content ==> n < |this.tblSeq|)
+          &&
+          forall k :: 0 <= k < |this.tblSeq| == this.tbl.Length ==> this.tblSeq[k] == this.tbl[k] == (k in this.content)
     }
       
-    constructor (size : nat) 
+    constructor(max_elem : nat) 
+      ensures |this.tblSeq| == max_elem + 1
+      ensures this.tbl.Length == |this.tblSeq|
       ensures this.Valid() && this.content == {} && this.footprint == {}
-      ensures |this.tblSeq| == size + 1
-      ensures forall k :: 0 <= k < |this.tblSeq| ==> this.tblSeq[k] == false
+      ensures forall k :: 0 <= k < |this.tblSeq| ==> this.tblSeq[k] == this.tbl[k] == false
+      ensures fresh(this.tbl)
     {
-      var aux := new bool[size + 1];
-      var i := 0;
-      while (i < aux.Length)
-        invariant 0 <= i <= aux.Length
-        invariant forall k :: 0 <= k < i ==> aux[k] == false
-      {
-        aux[i] := false;
-        i := i + 1;
-      }
+      var aux := new bool[max_elem + 1](_ => false); // last valid position must be aux[max_elem]. Lenght is max_elem + 1
+
       this.list := null;
       this.tbl := aux;
       this.tblSeq := aux[..];
@@ -65,24 +53,23 @@ module Ex5 {
       this.content := {};
     }
 
-    method mem (v : nat) returns (b : bool)
-      requires this.Valid() && v < |this.tblSeq|
-      ensures b == (v in this.content) 
-           && b == (tblSeq[v])
+    method mem(v : nat) returns (b : bool)
+      requires this.Valid()
+      requires v < |this.tblSeq|
+      ensures b == (v in this.content)
     {
-      b := false;
-      if (v < tbl.Length){
-        b := tbl[v];
-      }
+      b := this.tbl[v];
     }
     
-    method add (v : nat) 
+    method add(v : nat) 
       requires this.Valid()
       requires v < |this.tblSeq|
       ensures this.content == { v } + old(this.content)
+      ensures this.footprint == { this.list } + old(this.footprint)
       ensures this.Valid()
+      ensures fresh(this.footprint - old(this.footprint))
+      ensures this.tbl == old(this.tbl)
       modifies this, this.tbl
-
     {
       var value_exists := this.mem(v);
       if (this.list == null) {
@@ -92,41 +79,184 @@ module Ex5 {
         this.tblSeq := this.tbl[..];
         this.footprint := { aux };
         this.content := { v };
-      } else if (this.list != null && !value_exists) {
-        var added_node := this.list.add(v);
-        this.list := added_node;
-        this.tbl[v] := true;
-        this.tblSeq := tbl[..];
-        this.content := added_node.content;
-        this.footprint := added_node.footprint;
+      } 
+      else {
+        if (value_exists == false) {
+          var aux := this.list.add(v);
+          this.list := aux;
+          this.tbl[v] := true;
+          this.tblSeq := this.tbl[..];
+          this.content := aux.content;
+          this.footprint :=  aux.footprint;
+        }
+        else{
+          return;
+        }
       }
     }
 
     method union(s : Set) returns (r : Set)
-      requires this.Valid() && s.Valid()
-      ensures r.content == s.content + this.content
-      ensures r.footprint == s.footprint + this.footprint
-      ensures |r.tblSeq| == max(|this.tblSeq|, |s.tblSeq|)
+      requires this.Valid()
+      requires s.Valid()
 
-      ensures |this.tblSeq| >= |s.tblSeq| ==> 
-        (forall i :: 0 <= i < |s.tblSeq| ==> r.tblSeq[i] == this.tblSeq[i] || r.tblSeq[i])
-        &&
-        (forall i :: |s.tblSeq| <= i < |this.tblSeq| ==> r.tblSeq[i] == this.tblSeq[i])
-        
-      ensures |s.tblSeq| > |this.tblSeq| ==>
-        (forall i :: 0 <= i < |this.tblSeq| ==> r.tblSeq[i] == s.tblSeq[i] || r.tblSeq[i])
-        &&
-        (forall i :: |this.tblSeq| <= i < |s.tblSeq| ==> r.tblSeq[i] == s.tblSeq[i])
-
-      ensures fresh(r)
       ensures r.Valid()
+      ensures r.content == this.content + s.content
+      ensures fresh(r)
+      ensures forall k :: 0 <= k < |r.tblSeq| && k in this.content ==> r.tblSeq[k] == true
+      ensures forall k :: 0 <= k < |r.tblSeq| && k in s.content ==> r.tblSeq[k] == true
+      ensures forall k :: 0 <= k < |r.tblSeq| && r.tblSeq[k] == false ==> (k !in this.content) && (k !in s.content)
     {
+      // get max_element size
+      var max_elem;
+      var max_lenght := maxM(this.tbl.Length, s.tbl.Length);
+      if (max_lenght != 0) {
+         max_elem := max_lenght -1; // e.g. length is 3: [0,1,2] Max element is 2.
+      }
+      else {
+        max_elem := max_lenght;
+      }
+      r := new Set(max_elem);
+      
+      // calculate union
+      var curr := this.list;
+      ghost var seen_elements := {};
+
+      assert this.tbl.Length <= r.tbl.Length;
+      assert s.tbl.Length <= r.tbl.Length;
+      ghost var initialLength := r.tbl.Length;
+
+      while (curr != null)
+        decreases if curr != null then curr.footprint else {}
+        invariant r.Valid()
+        invariant s.Valid()
+        invariant r.tbl.Length == initialLength
+        invariant this.Valid()
+        invariant fresh(r) && fresh(r.tbl)
+        invariant curr != null ==> curr.Valid()
+        invariant this.tbl.Length <= r.tbl.Length
+        invariant r.content == seen_elements
+        invariant curr != null ==> this.content == curr.content + seen_elements
+        invariant curr == null ==> this.content == seen_elements
+      {
+        r.add(curr.val);
+        seen_elements := seen_elements + {curr.val};
+        curr := curr.next;
+      }
+
+      var curr_s := s.list;
+      ghost var seen_elements_s := {};
+
+      while (curr_s != null)
+        decreases if curr_s != null then curr_s.footprint else {}
+        invariant r.Valid()
+        invariant r.Valid()
+        invariant s.Valid()
+        invariant r.tbl.Length == initialLength
+        invariant this.Valid()
+        invariant fresh(r) && fresh(r.tbl)
+        invariant curr_s != null ==> curr_s.Valid()
+        invariant r.content == seen_elements_s + seen_elements
+        invariant s.tbl.Length <= r.tbl.Length
+        invariant curr_s != null ==> s.content == curr_s.content + seen_elements_s
+        invariant curr_s == null ==> s.content == seen_elements_s
+      {
+        r.add(curr_s.val);
+        seen_elements_s := seen_elements_s + { curr_s.val };
+        curr_s := curr_s.next;
+      }
     }
 
-    method inter(s : Set) returns (r : Set)
-    {
-    }
+    method inter(s: Set) returns (r : Set)
+      requires this.Valid()
+      requires s.Valid()
 
+      ensures r.Valid()
+      ensures r.content == this.content * s.content
+      ensures fresh(r)
+    {
+      var max_elem;
+      var max_length := maxM(this.tbl.Length, s.tbl.Length);
+      if (max_length != 0) {
+         max_elem := max_length -1; // e.g. length is 3: [0,1,2] Max element is 2.
+      }
+      else {
+        max_elem := max_length;
+      }
+      r := new Set(max_elem);
+
+      var curr := this.list;
+      ghost var added_elements := {};
+      ghost var seen_elements := {};
+
+      assert this.tbl.Length <= r.tbl.Length;
+      assert s.tbl.Length <= r.tbl.Length;
+      ghost var initialLength := r.tbl.Length;
+
+      while (curr != null) 
+        decreases if curr != null then curr.footprint else {}
+        invariant r.Valid()
+        invariant curr != null ==> curr.Valid()
+        invariant r.tbl.Length == initialLength
+        invariant this.Valid()
+        invariant fresh(r) && fresh(r.tbl)
+        invariant r.content == added_elements
+        invariant curr != null ==> this.content == curr.content + seen_elements
+        invariant curr == null ==> this.content == seen_elements
+
+        invariant seen_elements * s.content == added_elements
+
+        invariant forall x :: x in added_elements ==> x in this.content
+        invariant forall x :: x in added_elements ==> x in s.content
+      {
+        var also_in_s;
+
+        if (curr.val < s.tbl.Length){
+          also_in_s := s.mem(curr.val);
+        }
+        else{
+          also_in_s := false;
+        }
+        if (also_in_s) {
+          r.add(curr.val);
+          added_elements := added_elements + { curr.val };
+        }
+        seen_elements := seen_elements + { curr.val };
+        curr := curr.next;
+      }
+    }
   }
 
+  function maxF(x: nat, y: nat) : nat
+  {
+    if x >= y
+      then x
+      else y
+  }
+
+  method maxM(x: nat, y: nat) returns (z: nat) 
+    ensures z == maxF(x, y)
+  {
+    if (x >= y) {
+      z := x;
+    } else {
+      z := y;
+    }
+  }
+
+  function minF(x: nat, y: nat) : nat
+  {
+    if x <= y
+      then x
+      else y
+  }
+
+  method minM(x: nat, y: nat) returns (z: nat) 
+    ensures z == minF(x, y)
+  {
+    if (x <= y) {
+      z := x;
+    } else {
+      z := y;
+    }
+  }
 }
