davi_solutions/Ex3.dfy
@@ -1,121 +1,89 @@
-
 module Ex3 {
-
   class Node {
-
     var val : nat
     var next : Node?
 
-    ghost var footprint : set<Node> 
+    ghost var footprint : set<Node>
     ghost var content : set<nat>
 
-    ghost function Valid() : bool 
-      reads this, this.footprint 
+    ghost function Valid() : bool
+      reads this, this.footprint
       decreases footprint
     {
-      this in this.footprint 
+      this in this.footprint
       &&
       if (this.next == null)
-        then 
-          this.footprint == { this }
-          && 
-          this.content == { this.val }
-        else 
-          this.next in this.footprint
-          &&
-          this !in this.next.footprint
-          &&      
-          this.footprint == { this } + this.next.footprint 
-          &&
-          this.content == { this.val } + this.next.content
-          &&
-          this.next.Valid()
+      then
+        this.footprint == { this }
+        &&
+        this.content == { this.val }
+      else
+        this.next in this.footprint
+        &&
+        this !in this.next.footprint
+        &&
+        this.footprint == { this } + this.next.footprint
+        &&
+        this.content == { this.val } + this.next.content
+        &&
+        this.next.Valid()
     }
 
-    constructor (v : nat) 
+    constructor (v : nat)
       ensures this.Valid()
-      ensures this.content == { v } && this.footprint == { this }
+        && this.next == null && this.content == { v }
+        && this.footprint == { this } && this.val == v
     {
       this.val := v;
-      this.next := null;
+      this.next := null; 
       this.footprint := { this };
       this.content := { v };
-
     }
 
     method add(v : nat) returns (r : Node)
-      requires Valid()
+      requires this.Valid()
       ensures r.Valid()
-        && r.content== { v } + this.content
+        && r.content == { v } + this.content
         && r.footprint == { r } + this.footprint
       ensures r.next == this
+      ensures r.footprint - this.footprint == { r }
       ensures fresh(r)
-      ensures fresh(r.footprint - this.footprint)
+      // ensures fresh(r.footprint - this.footprint)
     {
       r := new Node(v);
       r.next := this;
-      r.content := { v } + this.content;
       r.footprint := { r } + this.footprint;
-
+      r.content := { v } + this.content;
     }
 
     method mem(v : nat) returns (b : bool)
-      requires Valid()
+      requires this.Valid()
       ensures b == (v in this.content)
-    {
-      var curr := this;
-      b := false;
-      ghost var list_aux := {};
-
-      while(curr != null)
-        invariant curr != null ==> curr.Valid()
-        invariant curr != null ==> this.content == list_aux + curr.content
-        invariant curr == null ==> this.content == list_aux
-        decreases if (curr != null) then curr.footprint else {}
-        invariant v !in list_aux
-      {
-        if(curr.val == v){
-          b := true;
-          return;
-        }
-        list_aux := list_aux + { curr.val };
-        curr := curr.next;
-      }
-  
-    }
-    method copy() returns (n : Node) 
-      requires Valid()
-      requires this.next != null ==> this.next.Valid()
-
-      ensures n.Valid()
-
-      ensures fresh(n)
-      ensures n.next != null ==> fresh(n.footprint)
-      
-      ensures n.next != null ==> n.footprint - n.next.footprint == { n }
-      ensures n.next == null ==> n.footprint == { n }
-      ensures n.content == this.content 
       decreases this.footprint
-    
+    {
+      b := false;
+      if (v == this.val) {
+        b := true; return;
+      } else if (this.next != null) {
+        b := this.next.mem(v); return;
+      }
+    }
+
+    method copy() returns (n : Node)
+      requires this.Valid()
+      ensures n.Valid()
+      ensures this.content == n.content
+      ensures |this.footprint| == |n.footprint|
+      ensures fresh(n.footprint)
+      decreases this.footprint
     {
       n := new Node(this.val);
-      
-      if (this.next != null)
-       {
+      if (this.next != null) {
         var aux := this.next.copy();
         n.next := aux;
         n.content := { n.val } + aux.content;
-        n.footprint := { n }  + aux.footprint;
-        return;
-      } else {
-        n.next := null;
-        n.content := { n.val };
-        n.footprint := { n };
-        return;
+        n.footprint := { n } + aux.footprint;
       }
-      return;
     }
   }
-
-  
 }
